Many random changes

Struct/DevTest.lean
@@ -1,1193 +1,148 @@
--- /-
--- Copyright (c) 2020 Microsoft Corporation. All rights reserved.
--- Released under Apache 2.0 license as described in the file LICENSE.
--- Authors: Leonardo de Moura, Sebastian Ullrich
--- -/
+-- Setup
+
+inductive Even : Nat → Prop
+| zero : Even Nat.zero
+| add_two : ∀ k : Nat, Even k → Even (k+2) 
+
+-- Example of existing structures
+example (hab : α ∧ β) : β ∨ α := by
+  exact Or.intro_right _ hab.left
+
+example (ha : α) : α := by
+  show α
+  . skip 
+    exact ha
+
+example (hab : α ∧ β) : β ∨ α := by
+  have ha : α := by exact hab.left
+  suffices α by
+    apply Or.intro_right _ _
+    exact this
+  show α
+  . exact ha
+  
+-- Example of intro, intros
+example : α₁ → α₂ ∧ α₃ → α₄ ∧ α₅ → α₆ ∧ α₇ → α₁ := by
+  intro ha1
+  intro (ha23 : α₂ ∧ α₃) ha45 (⟨ (ha6 : α₆), ha7⟩)
+  exact ha1
+
+-- Example of multiple goals
+example : α ↔ α := by
+  apply Iff.intro
+  case mp => intro ha ; exact ha
+  case mpr =>  intro ha ; exact ha
+
+-- Issue with multiple goals
+example : α ↔ α := by 
+  apply Iff.intro
+  focus
+    intro ha
+    exact ha
+  repeat {intro ha ; exact ha}
+
+
+
+-- Example of induction
+example (n : Nat) : n < n + 1 := by
+  induction n
+  repeat sorry
+example (n : Nat) : n < n + 1 := by
+  induction n 
+  case zero => sorry
+  case succ m m.ih => sorry
+example (n : Nat) : n < n + 1 := by
+  induction n with
+  | zero => sorry
+  | succ m m.ih => sorry
+
+example : α ↔ α := by
+  apply Iff.intro 
+  show α → α
+  . sorry
+  repeat sorry
+
+
+-- example : α ↔ α := by
+--   apply Iff.intro  
+--   case mp _ => note _ ; skip
+--   case mpr => skip
+
+  
+  -- State
+  -- Goal 1, case mp
+    -- α : Prop ⊢ α → α
+  -- Goal 2, case mpr 
+    -- α : Prop ⊢ α → α
+    -- sorry
+    -- sorry
+  -- { sorry }
+    -- sorry
+  -- . sorry
+
+example : α ↔ β := by
+  apply Iff.intro
+  show α → β
+
+-- CD01 - Changed context example
+example (ha : α) : α ∨ β := by
+  -- State: {α β : Prop, ha : α ⊢ α ∨ β }
+  apply Or.intro_left _ _
+  -- State: {α β : Prop, ha : α ⊢ α }
+  sorry
+example (ha : α) : α ∨ β := by
+  suffices α by
+    apply Or.intro_left _ _
+    exact this
+  sorry
+
+example (hab : β ∧ α) : α ∧ β := by
+  apply And.intro hab.right _
+  sorry
 
+example (n : Nat) : n = n := by
+  cases n <;> rfl
+  
+example : Even 6 := by
+  repeat apply Even.add_two _ _
+  sorry
 
 
+example (ha : α) : α := by
+  show α
+  . exact ha
 
--- namespace Lean.Elab.Tactic
--- open Meta
+example (ha : α) : α ∨ α := by
+  suffices α by
+    apply Or.intro_left _ _
+    exact this
+  sorry
 
--- /-
---   Given an `inductionAlt` of the form
---   ```
---   syntax inductionAltLHS := "| " (group("@"? ident) <|> hole) (ident <|> hole)*
---   syntax inductionAlt  := ppDedent(ppLine) inductionAltLHS+ " => " (hole <|> syntheticHole <|> tacticSeq)
---   ```
--- -/
--- private def getFirstAltLhs (alt : Syntax) : Syntax :=
---   alt[0][0]
--- /-- Return `inductionAlt` name. It assumes `alt` does not have multiple `inductionAltLHS` -/
--- private def getAltName (alt : Syntax) : Name :=
---   let lhs := getFirstAltLhs alt
---   if !lhs[1].isOfKind ``Parser.Term.hole then lhs[1][1].getId.eraseMacroScopes else `_
--- /-- Return `true` if the first LHS of the given alternative contains `@`. -/
--- private def altHasExplicitModifier (alt : Syntax) : Bool :=
---   let lhs := getFirstAltLhs alt
---   !lhs[1].isOfKind ``Parser.Term.hole && !lhs[1][0].isNone
--- /-- Return the variables in the first LHS of the given alternative. -/
--- private def getAltVars (alt : Syntax) : Array Syntax :=
---   let lhs := getFirstAltLhs alt
---   lhs[2].getArgs
--- /-- Return the variable names in the first LHS of the given alternative. -/
--- private def getAltVarNames (alt : Syntax) : Array Name :=
---   getAltVars  alt |>.map getNameOfIdent'
--- private def getAltRHS (alt : Syntax) : Syntax :=
---   alt[2]
--- private def getAltDArrow (alt : Syntax) : Syntax :=
---   alt[1]
+example (hab : α ∧ β) : α := by
+  have ha : α := by 
+    apply hab.left
+  sorry
 
--- -- Return true if `stx` is a term occurring in the RHS of the induction/cases tactic
--- def isHoleRHS (rhs : Syntax) : Bool :=
---   rhs.isOfKind ``Parser.Term.syntheticHole || rhs.isOfKind ``Parser.Term.hole
+example {α : Prop} :  α → β → α := by
+  -- State {α : Prop ⊢ α → α}
+  intros
+  -- State {α : Prop, ha : α ⊢ α}
+  assumption
 
--- def evalAlt (mvarId : MVarId) (alt : Syntax) (remainingGoals : Array MVarId) : TacticM (Array MVarId) :=
---   let rhs := getAltRHS alt
---   withCaseRef (getAltDArrow alt) rhs do
---     if isHoleRHS rhs then
---       let gs' ← mvarId.withContext <| withRef rhs do
---         let mvarDecl ← mvarId.getDecl
---         let val ← elabTermEnsuringType rhs mvarDecl.type
---         mvarId.assign val
---         let gs' ← getMVarsNoDelayed val
---         tagUntaggedGoals mvarDecl.userName `induction gs'.toList
---         pure gs'
---       return remainingGoals ++ gs'
---     else
---       setGoals [mvarId]
---       closeUsingOrAdmit (withTacticInfoContext alt (evalTactic rhs))
---       return remainingGoals
 
--- /-!
---   Helper method for creating an user-defined eliminator/recursor application.
--- -/
--- namespace ElimApp
+-- example (ha : α) : α := by
+--   show α by
+  -- .  exact ha
 
--- structure Context where
---   elimInfo : ElimInfo
---   targets  : Array Expr -- targets provided by the user
 
--- structure State where
---   argPos    : Nat := 0 -- current argument position
---   targetPos : Nat := 0 -- current target at targetsStx
---   f         : Expr
---   fType     : Expr
---   alts      : Array (Name × MVarId) := #[]
---   insts     : Array MVarId := #[]
+-- example : α → α  ↔ α := by
+--   apply Iff.intro
+--   intro _
+--   case mp h => sorry
 
--- abbrev M := ReaderT Context $ StateRefT State TermElabM
+example (n : Nat) : n = n := by
+  induction n with
+  | zero => ?_
+  | succ => ?_
+  sorry
 
--- private def addNewArg (arg : Expr) : M Unit :=
---   modify fun s => { s with argPos := s.argPos+1, f := mkApp s.f arg, fType := s.fType.bindingBody!.instantiate1 arg }
-
--- /-- Return the binder name at `fType`. This method assumes `fType` is a function type. -/
--- private def getBindingName : M Name := return (← get).fType.bindingName!
--- /-- Return the next argument expected type. This method assumes `fType` is a function type. -/
--- private def getArgExpectedType : M Expr := return (← get).fType.bindingDomain!
-
--- private def getFType : M Expr := do
---   let fType ← whnfForall (← get).fType
---   modify fun s => { s with fType := fType }
---   pure fType
-
--- structure Result where
---   elimApp : Expr
---   alts    : Array (Name × MVarId) := #[]
---   others  : Array MVarId := #[]
-
--- /--
---   Construct the an eliminator/recursor application. `targets` contains the explicit and implicit targets for
---   the eliminator. For example, the indices of builtin recursors are considered implicit targets.
---   Remark: the method `addImplicitTargets` may be used to compute the sequence of implicit and explicit targets
---   from the explicit ones.
--- -/
--- partial def mkElimApp (elimInfo : ElimInfo) (targets : Array Expr) (tag : Name) : TermElabM Result := do
---   let rec loop : M Unit := do
---     match (← getFType) with
---     | .forallE binderName _ _ c =>
---       let ctx ← read
---       let argPos := (← get).argPos
---       if ctx.elimInfo.motivePos == argPos then
---         let motive ← mkFreshExprMVar (← getArgExpectedType) MetavarKind.syntheticOpaque
---         addNewArg motive
---       else if ctx.elimInfo.targetsPos.contains argPos then
---         let s ← get
---         let ctx ← read
---         unless s.targetPos < ctx.targets.size do
---           throwError "insufficient number of targets for '{elimInfo.name}'"
---         let target := ctx.targets[s.targetPos]!
---         let expectedType ← getArgExpectedType
---         let target ← withAssignableSyntheticOpaque <| Term.ensureHasType expectedType target
---         modify fun s => { s with targetPos := s.targetPos + 1 }
---         addNewArg target
---       else match c with
---         | .implicit =>
---           let arg ← mkFreshExprMVar (← getArgExpectedType)
---           addNewArg arg
---         | .strictImplicit =>
---           let arg ← mkFreshExprMVar (← getArgExpectedType)
---           addNewArg arg
---         | .instImplicit =>
---           let arg ← mkFreshExprMVar (← getArgExpectedType) (kind := MetavarKind.synthetic) (userName := appendTag tag binderName)
---           modify fun s => { s with insts := s.insts.push arg.mvarId! }
---           addNewArg arg
---         | _ =>
---           let arg ← mkFreshExprSyntheticOpaqueMVar (← getArgExpectedType) (tag := appendTag tag binderName)
---           let x   ← getBindingName
---           modify fun s => { s with alts := s.alts.push (x, arg.mvarId!) }
---           addNewArg arg
---       loop
---     | _ =>
---       pure ()
---   let f ← Term.mkConst elimInfo.name
---   let fType ← inferType f
---   let (_, s) ← (loop).run { elimInfo := elimInfo, targets := targets } |>.run { f := f, fType := fType }
---   let mut others := #[]
---   for mvarId in s.insts do
---     try
---       unless (← Term.synthesizeInstMVarCore mvarId) do
---         mvarId.setKind .syntheticOpaque
---         others := others.push mvarId
---     catch _ =>
---       mvarId.setKind .syntheticOpaque
---       others := others.push mvarId
---   let alts ← s.alts.filterM fun alt => return !(← alt.2.isAssigned)
---   return { elimApp := (← instantiateMVars s.f), alts, others := others }
-
--- /-- Given a goal `... targets ... |- C[targets]` associated with `mvarId`, assign
---   `motiveArg := fun targets => C[targets]` -/
--- def setMotiveArg (mvarId : MVarId) (motiveArg : MVarId) (targets : Array FVarId) : MetaM Unit := do
---   let type ← inferType (mkMVar mvarId)
---   let motive ← mkLambdaFVars (targets.map mkFVar) type
---   let motiverInferredType ← inferType motive
---   let motiveType ← inferType (mkMVar motiveArg)
---   unless (← isDefEqGuarded motiverInferredType motiveType) do
---     throwError "type mismatch when assigning motive{indentExpr motive}\n{← mkHasTypeButIsExpectedMsg motiverInferredType motiveType}"
---   motiveArg.assign motive
-
--- private def getAltNumFields (elimInfo : ElimInfo) (altName : Name) : TermElabM Nat := do
---   for altInfo in elimInfo.altsInfo do
---     if altInfo.name == altName then
---       return altInfo.numFields
---   throwError "unknown alternative name '{altName}'"
-
--- private def checkAltNames (alts : Array (Name × MVarId)) (altsSyntax : Array Syntax) : TacticM Unit :=
---   for i in [:altsSyntax.size] do
---     let altStx := altsSyntax[i]!
---     if getAltName altStx == `_ && i != altsSyntax.size - 1 then
---       withRef altStx <| throwError "invalid occurrence of wildcard alternative, it must be the last alternative"
---     let altName := getAltName altStx
---     if altName != `_ then
---       unless alts.any fun (n, _) => n == altName do
---         throwErrorAt altStx "invalid alternative name '{altName}'"
-
--- /-- Given the goal `altMVarId` for a given alternative that introduces `numFields` new variables,
---     return the number of explicit variables. Recall that when the `@` is not used, only the explicit variables can
---     be named by the user. -/
--- private def getNumExplicitFields (altMVarId : MVarId) (numFields : Nat) : MetaM Nat := altMVarId.withContext do
---   let target ← altMVarId.getType
---   withoutModifyingState do
---     let (_, bis, _) ← forallMetaBoundedTelescope target numFields
---     return bis.foldl (init := 0) fun r bi => if bi.isExplicit then r + 1 else r
-
--- private def saveAltVarsInfo (altMVarId : MVarId) (altStx : Syntax) (fvarIds : Array FVarId) : TacticM Unit :=
---   withSaveInfoContext <| altMVarId.withContext do
---     let useNamesForExplicitOnly := !altHasExplicitModifier altStx
---     let mut i := 0
---     let altVars := getAltVars altStx
---     for fvarId in fvarIds do
---       if !useNamesForExplicitOnly || (← fvarId.getDecl).binderInfo.isExplicit then
---         if i < altVars.size then
---           Term.addLocalVarInfo altVars[i]! (mkFVar fvarId)
---           i := i + 1
-
--- /--
---   If `altsSyntax` is not empty we reorder `alts` using the order the alternatives have been provided
---   in `altsSyntax`. Motivations:
-
---   1- It improves the effectiveness of the `checkpoint` and `save` tactics. Consider the following example:
---   ```lean
---   example (h₁ : p ∨ q) (h₂ : p → x = 0) (h₃ : q → y = 0) : x * y = 0 := by
---     cases h₁ with
---     | inr h =>
---       sleep 5000 -- sleeps for 5 seconds
---       save
---       have : y = 0 := h₃ h
---       -- We can confortably work here
---     | inl h => stop ...
---   ```
---   If we do reorder, the `inl` alternative will be executed first. Moreover, as we type in the `inr` alternative,
---   type errors will "swallow" the `inl` alternative and affect the tactic state at `save` making it ineffective.
-
---   2- The errors are produced in the same order the appear in the code above. This is not super important when using IDEs.
--- -/
--- def reorderAlts (alts : Array (Name × MVarId)) (altsSyntax : Array Syntax) : Array (Name × MVarId) := Id.run do
---   if altsSyntax.isEmpty then
---     return alts
---   else
---     let mut alts := alts
---     let mut result := #[]
---     for altStx in altsSyntax do
---       let altName := getAltName altStx
---       let some i := alts.findIdx? (·.1 == altName) | return result ++ alts
---       result := result.push alts[i]!
---       alts := alts.eraseIdx i
---     return result ++ alts
-
--- -- TODO: Change myEvalAlts to return list of MVars
--- -- `getAltMVars` or something
--- def myEvalAlts (elimInfo : ElimInfo) (alts : Array (Name × MVarId)) (optPreTac : Syntax) (altsSyntax : Array Syntax)
---     (initialInfo : Info)
---     (numEqs : Nat := 0) (numGeneralized : Nat := 0) (toClear : Array FVarId := #[]) : TacticM Unit := do
---   checkAltNames alts altsSyntax
---   let hasAlts := altsSyntax.size > 0
---   if hasAlts then
---     -- default to initial state outside of alts
---     withInfoContext go (pure initialInfo)
---   else go
--- where
---   go := do
---     let alts := reorderAlts alts altsSyntax
---     let hasAlts := altsSyntax.size > 0
---     let mut usedWildcard := false
---     let mut subgoals := #[] -- when alternatives are not provided, we accumulate subgoals here
---     let mut altsSyntax := altsSyntax
-
---     -- TODO foreach, add mvar to list
---     for (altName, altMVarId) in alts do
---       trace[Elab.induction] "Alternative {altName}"
---       let numFields ← getAltNumFields elimInfo altName
---       let mut isWildcard := false
---       let altStx? ←
---         match altsSyntax.findIdx? (fun alt => getAltName alt == altName) with
---         | some idx =>
---           let altStx := altsSyntax[idx]!
---           altsSyntax := altsSyntax.eraseIdx idx
---           pure (some altStx)
---         | none => match altsSyntax.findIdx? (fun alt => getAltName alt == `_) with
---           | some idx =>
---             isWildcard := true
---             pure (some altsSyntax[idx]!)
---           | none =>
---             pure none
---       match altStx? with
---       | none =>
---         -- This is probably a match without any alternative syntax, all intro's are inaccessible anyways
---         let mut (_, altMVarId) ← altMVarId.introN numFields
---         match (← Cases.unifyEqs? numEqs altMVarId {}) with
---         | none   => pure () -- alternative is not reachable
---         | some (altMVarId', _) =>
---           (_, altMVarId) ← altMVarId'.introNP numGeneralized
---           for fvarId in toClear do
---             altMVarId ← altMVarId.tryClear fvarId
---           let altMVarIds ← applyPreTac altMVarId
---           if !hasAlts then
---             -- User did not provide alternatives using `|`
---             subgoals := subgoals ++ altMVarIds.toArray
---           else if altMVarIds.isEmpty then
---             pure ()
---           else
---             logError m!"alternative '{altName}' has not been provided"
---             altMVarIds.forM fun mvarId => admitGoal mvarId
---       | some altStx =>
---         trace[Elab.induction] "After creating altStx, I match on some altStx {altStx}"
---         (subgoals, usedWildcard) ← withRef altStx do
---           let unusedAlt :=
---             if isWildcard then
---               pure (#[], usedWildcard)
---             else
---               throwError "alternative '{altName}' is not needed"
---           let altVarNames := getAltVarNames altStx
---           let numFieldsToName ← if altHasExplicitModifier altStx then pure numFields else getNumExplicitFields altMVarId numFields
---           if altVarNames.size > numFieldsToName then
---             logError m!"too many variable names provided at alternative '{altName}', #{altVarNames.size} provided, but #{numFieldsToName} expected"
---           let mut (fvarIds, altMVarId) ← altMVarId.introN numFields altVarNames.toList (useNamesForExplicitOnly := !altHasExplicitModifier altStx)
-          
-          
---           -- NOTE TODO: This is actually the new goal post match statement
---           trace[Elab.induction] "Test01: {(← instantiateMVars (← altMVarId.getDecl).type)}"
---           altMVarId.withContext do
---             for ldecl in (← getLCtx) do
---               trace[Elab.induction] "Test02, {ldecl.userName}: {(← instantiateMVars ldecl.type)}"        
-
-
---           saveAltVarsInfo altMVarId altStx fvarIds
---           match (← Cases.unifyEqs? numEqs altMVarId {}) with
---           | none => unusedAlt
---           | some (altMVarId', _) =>
---             (_, altMVarId) ← altMVarId'.introNP numGeneralized
---             for fvarId in toClear do
---               altMVarId ← altMVarId.tryClear fvarId
---             let altMVarIds ← applyPreTac altMVarId
---             if altMVarIds.isEmpty then
---               unusedAlt
---             else
---               let mut subgoals := subgoals
---               for altMVarId' in altMVarIds do
---                 altMVarId'.withContext do
---                   trace[Elab.induction] m!"Test03, {(← instantiateMVars (← altMVarId'.getDecl).type)}"
---                   altMVarId'.withContext do
---                     for ldecl in (← getLCtx) do
---                       trace[Elab.induction] "Test04, {ldecl.userName}: {(← instantiateMVars ldecl.type)}"  
-
-
---                 subgoals ← evalAlt altMVarId' altStx subgoals
---               pure (subgoals, usedWildcard || isWildcard)          
---     if usedWildcard then
---       altsSyntax := altsSyntax.filter fun alt => getAltName alt != `_
---     unless altsSyntax.isEmpty do
---       logErrorAt altsSyntax[0]! "unused alternative"
---     for goal in subgoals do
---       trace[Elab.induction] m!"TEST: {(← instantiateMVars (← goal.getDecl).type)}"
---     setGoals subgoals.toList
---   applyPreTac (mvarId : MVarId) : TacticM (List MVarId) :=
---     if optPreTac.isNone then do
---       return [mvarId]
---     else
---       evalTacticAt optPreTac[0] mvarId
-
--- end ElimApp
-
--- /-
---   Recall that
---   ```
---   generalizingVars := optional (" generalizing " >> many1 ident)
---   «induction»  := leading_parser nonReservedSymbol "induction " >> majorPremise >> usingRec >> generalizingVars >> optional inductionAlts
---   ```
---   `stx` is syntax for `induction`. -/
--- private def getUserGeneralizingFVarIds (stx : Syntax) : TacticM (Array FVarId) :=
---   withRef stx do
---     let generalizingStx := stx[3]
---     if generalizingStx.isNone then
---       pure #[]
---     else
---       trace[Elab.induction] "{generalizingStx}"
---       let vars := generalizingStx[1].getArgs
---       getFVarIds vars
-
--- -- process `generalizingVars` subterm of induction Syntax `stx`.
--- private def generalizeVars (mvarId : MVarId) (stx : Syntax) (targets : Array Expr) : TacticM (Nat × MVarId) :=
---   mvarId.withContext do
---     let userFVarIds ← getUserGeneralizingFVarIds stx
---     let forbidden ← mkGeneralizationForbiddenSet targets
---     let mut s ← getFVarSetToGeneralize targets forbidden
---     for userFVarId in userFVarIds do
---       if forbidden.contains userFVarId then
---         throwError "variable cannot be generalized because target depends on it{indentExpr (mkFVar userFVarId)}"
---       if s.contains userFVarId then
---         throwError "unnecessary 'generalizing' argument, variable '{mkFVar userFVarId}' is generalized automatically"
---       s := s.insert userFVarId
---     let fvarIds ← sortFVarIds s.toArray
---     let (fvarIds, mvarId') ← mvarId.revert fvarIds
---     return (fvarIds.size, mvarId')
-
--- /--
--- Given `inductionAlts` of the fom
--- ```
--- syntax inductionAlts := "with " (tactic)? withPosition( (colGe inductionAlt)+)
--- ```
--- Return an array containing its alternatives.
--- -/
--- private def getAltsOfInductionAlts (inductionAlts : Syntax) : Array Syntax :=
---   inductionAlts[2].getArgs
-
--- private def getAltsOfOptInductionAlts (optInductionAlts : Syntax) : Array Syntax :=
---   if optInductionAlts.isNone then #[] else getAltsOfInductionAlts optInductionAlts[0]
-
--- private def getOptPreTacOfOptInductionAlts (optInductionAlts : Syntax) : Syntax :=
---   if optInductionAlts.isNone then mkNullNode else optInductionAlts[0][1]
-
--- private def isMultiAlt (alt : Syntax) : Bool :=
---   alt[0].getNumArgs > 1
-
--- /-- Return `some #[alt_1, ..., alt_n]` if `alt` has multiple LHSs. -/
--- private def expandMultiAlt? (alt : Syntax) : Option (Array Syntax) := Id.run do
---   if isMultiAlt alt then
---     some <| alt[0].getArgs.map fun lhs => alt.setArg 0 (mkNullNode #[lhs])
---   else
---     none
-
--- /--
--- Given `inductionAlts` of the form
--- ```
--- syntax inductionAlts := "with " (tactic)? withPosition( (colGe inductionAlt)+)
--- ```
--- Return `some inductionAlts'` if one of the alternatives have multiple LHSs, in the new `inductionAlts'`
--- all alternatives have a single LHS.
-
--- Remark: the `RHS` of alternatives with multi LHSs is copied.
--- -/
--- private def expandInductionAlts? (inductionAlts : Syntax) : Option Syntax := Id.run do
---   let alts := getAltsOfInductionAlts inductionAlts
---   if alts.any isMultiAlt then
---     let mut altsNew := #[]
---     for alt in alts do
---       if let some alt' := expandMultiAlt? alt then
---         altsNew := altsNew ++ alt'
---       else
---         altsNew := altsNew.push alt
---     some <| inductionAlts.setArg 2 (mkNullNode altsNew)
---   else
---     none
-
--- /--
--- Expand
--- ```
--- syntax "induction " term,+ (" using " ident)?  ("generalizing " (colGt term:max)+)? (inductionAlts)? : tactic
--- ```
--- if `inductionAlts` has an alternative with multiple LHSs.
--- -/
--- private def expandInduction? (induction : Syntax) : Option Syntax := do
---   let optInductionAlts := induction[4]
---   guard <| !optInductionAlts.isNone
---   let inductionAlts' ← expandInductionAlts? optInductionAlts[0]
---   return induction.setArg 4 (mkNullNode #[inductionAlts'])
-
--- /--
--- Expand
--- ```
--- syntax "cases " casesTarget,+ (" using " ident)? (inductionAlts)? : tactic
--- ```
--- if `inductionAlts` has an alternative with multiple LHSs.
--- -/
--- private def expandCases? (induction : Syntax) : Option Syntax := do
---   let optInductionAlts := induction[3]
---   guard <| !optInductionAlts.isNone
---   let inductionAlts' ← expandInductionAlts? optInductionAlts[0]
---   return induction.setArg 3 (mkNullNode #[inductionAlts'])
-
--- /--
---   We may have at most one `| _ => ...` (wildcard alternative), and it must not set variable names.
---   The idea is to make sure users do not write unstructured tactics. -/
--- private def checkAltsOfOptInductionAlts (optInductionAlts : Syntax) : TacticM Unit :=
---   unless optInductionAlts.isNone do
---     let mut found := false
---     for alt in getAltsOfInductionAlts optInductionAlts[0] do
---       let n := getAltName alt
---       if n == `_ then
---         unless (getAltVarNames alt).isEmpty do
---           throwErrorAt alt "wildcard alternative must not specify variable names"
---         if found then
---           throwErrorAt alt "more than one wildcard alternative '| _ => ...' used"
---         found := true
-
--- def getInductiveValFromMajor (major : Expr) : TacticM InductiveVal :=
---   liftMetaMAtMain fun mvarId => do
---     let majorType ← inferType major
---     let majorType ← whnf majorType
---     matchConstInduct majorType.getAppFn
---       (fun _ => Meta.throwTacticEx `induction mvarId m!"major premise type is not an inductive type {indentExpr majorType}")
---       (fun val _ => pure val)
-
--- -- `optElimId` is of the form `("using" ident)?`
--- private def getElimNameInfo (optElimId : Syntax) (targets : Array Expr) (induction : Bool): TacticM ElimInfo := do
---   if optElimId.isNone then
---     if let some elimInfo ← getCustomEliminator? targets then
---       return elimInfo
---     unless targets.size == 1 do
---       throwError "eliminator must be provided when multiple targets are used (use 'using <eliminator-name>'), and no default eliminator has been registered using attribute `[eliminator]`"
---     let indVal ← getInductiveValFromMajor targets[0]!
---     if induction && indVal.all.length != 1 then
---       throwError "'induction' tactic does not support mutually inductive types, the eliminator '{mkRecName indVal.name}' has multiple motives"
---     if induction && indVal.isNested then
---       throwError "'induction' tactic does not support nested inductive types, the eliminator '{mkRecName indVal.name}' has multiple motives"
---     let elimName := if induction then mkRecName indVal.name else mkCasesOnName indVal.name
---     getElimInfo elimName
---   else
---     let elimId := optElimId[1]
---     let elimName ← withRef elimId do resolveGlobalConstNoOverloadWithInfo elimId
---     withRef elimId <| getElimInfo elimName
-
--- private def shouldGeneralizeTarget (e : Expr) : MetaM Bool := do
---   if let .fvar fvarId .. := e then
---     return (←  fvarId.getDecl).hasValue -- must generalize let-decls
---   else
---     return true
-
--- private def generalizeTargets (exprs : Array Expr) : TacticM (Array Expr) := do
---   if (← withMainContext <| exprs.anyM (shouldGeneralizeTarget ·)) then
---     liftMetaTacticAux fun mvarId => do
---       let (fvarIds, mvarId) ← mvarId.generalize (exprs.map fun expr => { expr })
---       return (fvarIds.map mkFVar, [mvarId])
---   else
---     return exprs
-
--- def myEvalInduction : Tactic := fun stx =>
---   match expandInduction? stx with
---   | some stxNew => withMacroExpansion stx stxNew <| evalTactic stxNew
---   | _ => focus do
---     let optInductionAlts := stx[4]
---     let alts := getAltsOfOptInductionAlts optInductionAlts
---     let targets ← withMainContext <| stx[1].getSepArgs.mapM (elabTerm · none)
---     let targets ← generalizeTargets targets
---     let elimInfo ← withMainContext <| getElimNameInfo stx[2] targets (induction := true)
---     let mvarId ← getMainGoal
---     -- save initial info before main goal is reassigned
---     let initInfo ← mkTacticInfo (← getMCtx) (← getUnsolvedGoals) (← getRef)
---     let tag ← mvarId.getTag
---     mvarId.withContext do
---       let targets ← addImplicitTargets elimInfo targets
---       checkTargets targets
---       let targetFVarIds := targets.map (·.fvarId!)
---       let (n, mvarId) ← generalizeVars mvarId stx targets
---       mvarId.withContext do
---         let result ← withRef stx[1] do -- use target position as reference
---           ElimApp.mkElimApp elimInfo targets tag
---         trace[Elab.induction] "elimApp: {result.elimApp}"
-        
---         -- let x ← result.alts.mapM (fun (name, mvar) => do
---         --   let y ← mvar.getDecl
---         --   let z ← instantiateMVars y.type
---         --   trace[Elab.induction] "{name}: {z}"
---         --   for ldecl in y.lctx do
---         --     trace[Elab.induction] "alts, {ldecl.userName}: {(← instantiateMVars ldecl.type)}"
---         --   )
---         -- let x ← result.others.mapM (fun mvar => do
---         --   let y ← mvar.getDecl
---         --   let z ← instantiateMVars y.type
---         --   trace[Elab.induction] "_: {z}"
---         --   for ldecl in y.lctx do
---         --     trace[Elab.induction] "others, {ldecl.userName}: {(← instantiateMVars ldecl.type)}"
---         --   )
-
---         let elimArgs := result.elimApp.getAppArgs
---         ElimApp.setMotiveArg mvarId elimArgs[elimInfo.motivePos]!.mvarId! targetFVarIds
---         let optPreTac := getOptPreTacOfOptInductionAlts optInductionAlts
-
---         mvarId.assign result.elimApp
-
---         -- mvarId.withContext do
---         --   for ldecl in (← getLCtx) do
---         --     trace[Elab.induction] "test, {ldecl.userName}: {(← instantiateMVars ldecl.type)}"
-
---         ElimApp.myEvalAlts elimInfo result.alts optPreTac alts initInfo (numGeneralized := n) (toClear := targetFVarIds)
---         appendGoals result.others.toList
--- where
---   checkTargets (targets : Array Expr) : MetaM Unit := do
---     let mut foundFVars : FVarIdSet := {}
---     for target in targets do
---       unless target.isFVar do
---         throwError "index in target's type is not a variable (consider using the `cases` tactic instead){indentExpr target}"
---       if foundFVars.contains target.fvarId! then
---         throwError "target (or one of its indices) occurs more than once{indentExpr target}"
-
--- def elabCasesTargets (targets : Array Syntax) : TacticM (Array Expr) :=
---   withMainContext do
---     let args ← targets.mapM fun target => do
---       let hName? := if target[0].isNone then none else some target[0][0].getId
---       let expr ← elabTerm target[1] none
---       return { expr, hName? : GeneralizeArg }
---     if (← withMainContext <| args.anyM fun arg => shouldGeneralizeTarget arg.expr <||> pure arg.hName?.isSome) then
---       liftMetaTacticAux fun mvarId => do
---         let argsToGeneralize ← args.filterM fun arg => shouldGeneralizeTarget arg.expr <||> pure arg.hName?.isSome
---         let (fvarIdsNew, mvarId) ← mvarId.generalize argsToGeneralize
---         let mut result := #[]
---         let mut j := 0
---         for arg in args do
---           if (← shouldGeneralizeTarget arg.expr) || arg.hName?.isSome then
---             result := result.push (mkFVar fvarIdsNew[j]!)
---             j := j+1
---           else
---             result := result.push arg.expr
---         return (result, [mvarId])
---     else
---       return args.map (·.expr)
-
--- def myEvalCases : Tactic := fun stx =>
---   match expandCases? stx with
---   | some stxNew => withMacroExpansion stx stxNew <| evalTactic stxNew
---   | _ => focus do
---     -- leading_parser nonReservedSymbol "cases " >> sepBy1 (group majorPremise) ", " >> usingRec >> optInductionAlts
---     let targets ← elabCasesTargets stx[1].getSepArgs
---     let optInductionAlts := stx[3]
---     let optPreTac := getOptPreTacOfOptInductionAlts optInductionAlts
---     let alts :=  getAltsOfOptInductionAlts optInductionAlts
---     let targetRef := stx[1]
---     let elimInfo ← withMainContext <| getElimNameInfo stx[2] targets (induction := false)
---     let mvarId ← getMainGoal
---     -- save initial info before main goal is reassigned
---     let initInfo ← mkTacticInfo (← getMCtx) (← getUnsolvedGoals) (← getRef)
---     let tag ← mvarId.getTag
---     mvarId.withContext do
---       let targets ← addImplicitTargets elimInfo targets
---       let result ← withRef targetRef <| ElimApp.mkElimApp elimInfo targets tag
---       let elimArgs := result.elimApp.getAppArgs
---       let targets ← elimInfo.targetsPos.mapM fun i => instantiateMVars elimArgs[i]!
---       let motiveType ← inferType elimArgs[elimInfo.motivePos]!
---       let mvarId ← generalizeTargetsEq mvarId motiveType targets
---       let (targetsNew, mvarId) ← mvarId.introN targets.size
-
---       mvarId.withContext do
---         ElimApp.setMotiveArg mvarId elimArgs[elimInfo.motivePos]!.mvarId! targetsNew
---         mvarId.assign result.elimApp
---         ElimApp.myEvalAlts elimInfo result.alts optPreTac alts initInfo (numEqs := targets.size) (toClear := targetsNew)
-
--- builtin_initialize
---   registerTraceClass `Elab.cases
---   registerTraceClass `Elab.induction
-
--- open
---   Lean.Parser.Tactic
-
--- elab &"myTestTactic " t:term " : " t2:ident  " : " t3:(ident) : tactic => do
---   let case1 := mkIdent "zero"
---   let case2 := mkIdent "succ"
---   let indAlt1 ← `(inductionAlt| | $case1 => sorry)
---   let indAlt2 ← `(inductionAlt| | $case2 $t2 $t3 => sorry)
---   myEvalInduction (← `(tactic|induction $t with $indAlt1:inductionAlt $indAlt2:inductionAlt))
-
--- elab &"myTestTactic2 " t:casesTarget " : " t2:ident : tactic => do
---   let case1 := mkIdent "zero"
---   let case2 := mkIdent "succ"
---   let indAlt1 ← `(inductionAlt| | $case1 => sorry)
---   let indAlt2 ← `(inductionAlt| | $case2 $t2 => sorry)
---   myEvalCases (← `(tactic|cases $t with $indAlt1:inductionAlt $indAlt2:inductionAlt))
-
-
--- end Lean.Elab.Tactic
-
-
--- set_option trace.Elab.induction true
--- set_option pp.rawOnError true
-
--- example (n : Nat) : n = n := by
---   -- Q : Why do goals contain _uniq, even if the relevant mvar seems named in ldecls?
---   myTestTactic (n) : m : m.ih 
---   -- myTestTactic2 (n) : m
---   -- cases n with
---   -- | zero => sorry
---   -- | succ m => sorry
---   -- repeat admit
-
-
-import Lean.Util.CollectFVars
-import Lean.Parser.Term
-import Lean.Meta.RecursorInfo
-import Lean.Meta.CollectMVars
-import Lean.Meta.Tactic.ElimInfo
-import Lean.Meta.Tactic.Induction
-import Lean.Meta.Tactic.Cases
-import Lean.Meta.GeneralizeVars
-import Lean.Elab.App
-import Lean.Elab.Tactic.ElabTerm
-import Lean.Elab.Tactic.Generalize
-
-namespace InductionHelper
-
-open 
-  Lean 
-  Lean.Expr
-  Lean.Meta 
-  Lean.Elab
-  Lean.Elab.Tactic
-  Lean.PrettyPrinter 
-
--- # Necessary duplicate (private) helper functions from Lean.Elab.Tactic.induction from nightly-2022-08-09
--- # Removed most comments, removed namespaces
-private def getFirstAltLhs (alt : Syntax) : Syntax :=
-  alt[0][0]
-private def getAltName (alt : Syntax) : Name :=
-  let lhs := getFirstAltLhs alt
-  if !lhs[1].isOfKind ``Parser.Term.hole then lhs[1][1].getId.eraseMacroScopes else `_
-private def altHasExplicitModifier (alt : Syntax) : Bool :=
-  let lhs := getFirstAltLhs alt
-  !lhs[1].isOfKind ``Parser.Term.hole && !lhs[1][0].isNone
-private def getAltVars (alt : Syntax) : Array Syntax :=
-  let lhs := getFirstAltLhs alt
-  lhs[2].getArgs
-private def getAltVarNames (alt : Syntax) : Array Name :=
-  getAltVars  alt |>.map getNameOfIdent'
-private def getAltRHS (alt : Syntax) : Syntax :=
-  alt[2]
-private def getAltDArrow (alt : Syntax) : Syntax :=
-  alt[1]
-
-def isHoleRHS (rhs : Syntax) : Bool :=
-  rhs.isOfKind ``Parser.Term.syntheticHole || rhs.isOfKind ``Parser.Term.hole
-
-def evalAlt (mvarId : MVarId) (alt : Syntax) (remainingGoals : Array MVarId) : TacticM (Array MVarId) :=
-  let rhs := getAltRHS alt
-  withCaseRef (getAltDArrow alt) rhs do
-    if isHoleRHS rhs then
-      let gs' ← mvarId.withContext <| withRef rhs do
-        let mvarDecl ← mvarId.getDecl
-        let val ← elabTermEnsuringType rhs mvarDecl.type
-        mvarId.assign val
-        let gs' ← getMVarsNoDelayed val
-        tagUntaggedGoals mvarDecl.userName `induction gs'.toList
-        pure gs'
-      return remainingGoals ++ gs'
-    else
-      setGoals [mvarId]
-      closeUsingOrAdmit (withTacticInfoContext alt (evalTactic rhs))
-      return remainingGoals
-
-structure Context where
-  elimInfo : ElimInfo
-  targets  : Array Expr -- targets provided by the user
-
-structure State where
-  argPos    : Nat := 0 -- current argument position
-  targetPos : Nat := 0 -- current target at targetsStx
-  f         : Expr
-  fType     : Expr
-  alts      : Array (Name × MVarId) := #[]
-  insts     : Array MVarId := #[]
-
-abbrev M := ReaderT Context $ StateRefT State TermElabM
-
-private def addNewArg (arg : Expr) : M Unit :=
-  modify fun s => { s with argPos := s.argPos+1, f := mkApp s.f arg, fType := s.fType.bindingBody!.instantiate1 arg }
-
-private def getBindingName : M Name := return (← get).fType.bindingName!
-private def getArgExpectedType : M Expr := return (← get).fType.bindingDomain!
-
-private def getFType : M Expr := do
-  let fType ← whnfForall (← get).fType
-  modify fun s => { s with fType := fType }
-  pure fType
-
-structure Result where
-  elimApp : Expr
-  alts    : Array (Name × MVarId) := #[]
-  others  : Array MVarId := #[]
-
-partial def mkElimApp (elimInfo : ElimInfo) (targets : Array Expr) (tag : Name) : TermElabM Result := do
-  let rec loop : M Unit := do
-    match (← getFType) with
-    | .forallE binderName _ _ c =>
-      let ctx ← read
-      let argPos := (← get).argPos
-      if ctx.elimInfo.motivePos == argPos then
-        let motive ← mkFreshExprMVar (← getArgExpectedType) MetavarKind.syntheticOpaque
-        addNewArg motive
-      else if ctx.elimInfo.targetsPos.contains argPos then
-        let s ← get
-        let ctx ← read
-        unless s.targetPos < ctx.targets.size do
-          throwError "insufficient number of targets for '{elimInfo.name}'"
-        let target := ctx.targets[s.targetPos]!
-        let expectedType ← getArgExpectedType
-        let target ← withAssignableSyntheticOpaque <| Term.ensureHasType expectedType target
-        modify fun s => { s with targetPos := s.targetPos + 1 }
-        addNewArg target
-      else match c with
-        | .implicit =>
-          let arg ← mkFreshExprMVar (← getArgExpectedType)
-          addNewArg arg
-        | .strictImplicit =>
-          let arg ← mkFreshExprMVar (← getArgExpectedType)
-          addNewArg arg
-        | .instImplicit =>
-          let arg ← mkFreshExprMVar (← getArgExpectedType) (kind := MetavarKind.synthetic) (userName := appendTag tag binderName)
-          modify fun s => { s with insts := s.insts.push arg.mvarId! }
-          addNewArg arg
-        | _ =>
-          let arg ← mkFreshExprSyntheticOpaqueMVar (← getArgExpectedType) (tag := appendTag tag binderName)
-          let x   ← getBindingName
-          modify fun s => { s with alts := s.alts.push (x, arg.mvarId!) }
-          addNewArg arg
-      loop
-    | _ =>
-      pure ()
-  let f ← Term.mkConst elimInfo.name
-  let fType ← inferType f
-  let (_, s) ← (loop).run { elimInfo := elimInfo, targets := targets } |>.run { f := f, fType := fType }
-  let mut others := #[]
-  for mvarId in s.insts do
-    try
-      unless (← Term.synthesizeInstMVarCore mvarId) do
-        mvarId.setKind .syntheticOpaque
-        others := others.push mvarId
-    catch _ =>
-      mvarId.setKind .syntheticOpaque
-      others := others.push mvarId
-  let alts ← s.alts.filterM fun alt => return !(← alt.2.isAssigned)
-  return { elimApp := (← instantiateMVars s.f), alts, others := others }
-
-def setMotiveArg (mvarId : MVarId) (motiveArg : MVarId) (targets : Array FVarId) : MetaM Unit := do
-  let type ← inferType (mkMVar mvarId)
-  let motive ← mkLambdaFVars (targets.map mkFVar) type
-  let motiverInferredType ← inferType motive
-  let motiveType ← inferType (mkMVar motiveArg)
-  unless (← isDefEqGuarded motiverInferredType motiveType) do
-    throwError "type mismatch when assigning motive{indentExpr motive}\n{← mkHasTypeButIsExpectedMsg motiverInferredType motiveType}"
-  motiveArg.assign motive
-
-private def getAltNumFields (elimInfo : ElimInfo) (altName : Name) : TermElabM Nat := do
-  for altInfo in elimInfo.altsInfo do
-    if altInfo.name == altName then
-      return altInfo.numFields
-  throwError "unknown alternative name '{altName}'"
-
-private def checkAltNames (alts : Array (Name × MVarId)) (altsSyntax : Array Syntax) : TacticM Unit :=
-  for i in [:altsSyntax.size] do
-    let altStx := altsSyntax[i]!
-    if getAltName altStx == `_ && i != altsSyntax.size - 1 then
-      withRef altStx <| throwError "invalid occurrence of wildcard alternative, it must be the last alternative"
-    let altName := getAltName altStx
-    if altName != `_ then
-      unless alts.any fun (n, _) => n == altName do
-        throwErrorAt altStx "invalid alternative name '{altName}'"
-
-private def getNumExplicitFields (altMVarId : MVarId) (numFields : Nat) : MetaM Nat := altMVarId.withContext do
-  let target ← altMVarId.getType
-  withoutModifyingState do
-    let (_, bis, _) ← forallMetaBoundedTelescope target numFields
-    return bis.foldl (init := 0) fun r bi => if bi.isExplicit then r + 1 else r
-
-private def saveAltVarsInfo (altMVarId : MVarId) (altStx : Syntax) (fvarIds : Array FVarId) : TacticM Unit :=
-  withSaveInfoContext <| altMVarId.withContext do
-    let useNamesForExplicitOnly := !altHasExplicitModifier altStx
-    let mut i := 0
-    let altVars := getAltVars altStx
-    for fvarId in fvarIds do
-      if !useNamesForExplicitOnly || (← fvarId.getDecl).binderInfo.isExplicit then
-        if i < altVars.size then
-          Term.addLocalVarInfo altVars[i]! (mkFVar fvarId)
-          i := i + 1
-
-def reorderAlts (alts : Array (Name × MVarId)) (altsSyntax : Array Syntax) : Array (Name × MVarId) := Id.run do
-  if altsSyntax.isEmpty then
-    return alts
-  else
-    let mut alts := alts
-    let mut result := #[]
-    for altStx in altsSyntax do
-      let altName := getAltName altStx
-      let some i := alts.findIdx? (·.1 == altName) | return result ++ alts
-      result := result.push alts[i]!
-      alts := alts.eraseIdx i
-    return result ++ alts
-
-private def getUserGeneralizingFVarIds (stx : Syntax) : TacticM (Array FVarId) :=
-  withRef stx do
-    let generalizingStx := stx[3]
-    if generalizingStx.isNone then
-      pure #[]
-    else
-      trace[Elab.induction] "{generalizingStx}"
-      let vars := generalizingStx[1].getArgs
-      getFVarIds vars
-
-private def generalizeVars (mvarId : MVarId) (stx : Syntax) (targets : Array Expr) : TacticM (Nat × MVarId) :=
-  mvarId.withContext do
-    let userFVarIds ← getUserGeneralizingFVarIds stx
-    let forbidden ← mkGeneralizationForbiddenSet targets
-    let mut s ← getFVarSetToGeneralize targets forbidden
-    for userFVarId in userFVarIds do
-      if forbidden.contains userFVarId then
-        throwError "variable cannot be generalized because target depends on it{indentExpr (mkFVar userFVarId)}"
-      if s.contains userFVarId then
-        throwError "unnecessary 'generalizing' argument, variable '{mkFVar userFVarId}' is generalized automatically"
-      s := s.insert userFVarId
-    let fvarIds ← sortFVarIds s.toArray
-    let (fvarIds, mvarId') ← mvarId.revert fvarIds
-    return (fvarIds.size, mvarId')
-
-private def getAltsOfInductionAlts (inductionAlts : Syntax) : Array Syntax :=
-  inductionAlts[2].getArgs
-
-private def getAltsOfOptInductionAlts (optInductionAlts : Syntax) : Array Syntax :=
-  if optInductionAlts.isNone then #[] else getAltsOfInductionAlts optInductionAlts[0]
-
-private def getOptPreTacOfOptInductionAlts (optInductionAlts : Syntax) : Syntax :=
-  if optInductionAlts.isNone then mkNullNode else optInductionAlts[0][1]
-
-private def isMultiAlt (alt : Syntax) : Bool :=
-  alt[0].getNumArgs > 1
-
-/-- Return `some #[alt_1, ..., alt_n]` if `alt` has multiple LHSs. -/
-private def expandMultiAlt? (alt : Syntax) : Option (Array Syntax) := Id.run do
-  if isMultiAlt alt then
-    some <| alt[0].getArgs.map fun lhs => alt.setArg 0 (mkNullNode #[lhs])
-  else
-    none
-
-private def expandInductionAlts? (inductionAlts : Syntax) : Option Syntax := Id.run do
-  let alts := getAltsOfInductionAlts inductionAlts
-  if alts.any isMultiAlt then
-    let mut altsNew := #[]
-    for alt in alts do
-      if let some alt' := expandMultiAlt? alt then
-        altsNew := altsNew ++ alt'
-      else
-        altsNew := altsNew.push alt
-    some <| inductionAlts.setArg 2 (mkNullNode altsNew)
-  else
-    none
-
-private def expandInduction? (induction : Syntax) : Option Syntax := do
-  let optInductionAlts := induction[4]
-  guard <| !optInductionAlts.isNone
-  let inductionAlts' ← expandInductionAlts? optInductionAlts[0]
-  return induction.setArg 4 (mkNullNode #[inductionAlts'])
-
-private def expandCases? (induction : Syntax) : Option Syntax := do
-  let optInductionAlts := induction[3]
-  guard <| !optInductionAlts.isNone
-  let inductionAlts' ← expandInductionAlts? optInductionAlts[0]
-  return induction.setArg 3 (mkNullNode #[inductionAlts'])
-
-private def checkAltsOfOptInductionAlts (optInductionAlts : Syntax) : TacticM Unit :=
-  unless optInductionAlts.isNone do
-    let mut found := false
-    for alt in getAltsOfInductionAlts optInductionAlts[0] do
-      let n := getAltName alt
-      if n == `_ then
-        unless (getAltVarNames alt).isEmpty do
-          throwErrorAt alt "wildcard alternative must not specify variable names"
-        if found then
-          throwErrorAt alt "more than one wildcard alternative '| _ => ...' used"
-        found := true
-
-def getInductiveValFromMajor (major : Expr) : TacticM InductiveVal :=
-  liftMetaMAtMain fun mvarId => do
-    let majorType ← inferType major
-    let majorType ← whnf majorType
-    matchConstInduct majorType.getAppFn
-      (fun _ => Meta.throwTacticEx `induction mvarId m!"major premise type is not an inductive type {indentExpr majorType}")
-      (fun val _ => pure val)
-
-private def getElimNameInfo (optElimId : Syntax) (targets : Array Expr) (induction : Bool): TacticM ElimInfo := do
-  if optElimId.isNone then
-    if let some elimInfo ← getCustomEliminator? targets then
-      return elimInfo
-    unless targets.size == 1 do
-      throwError "eliminator must be provided when multiple targets are used (use 'using <eliminator-name>'), and no default eliminator has been registered using attribute `[eliminator]`"
-    let indVal ← getInductiveValFromMajor targets[0]!
-    if induction && indVal.all.length != 1 then
-      throwError "'induction' tactic does not support mutually inductive types, the eliminator '{mkRecName indVal.name}' has multiple motives"
-    if induction && indVal.isNested then
-      throwError "'induction' tactic does not support nested inductive types, the eliminator '{mkRecName indVal.name}' has multiple motives"
-    let elimName := if induction then mkRecName indVal.name else mkCasesOnName indVal.name
-    getElimInfo elimName
-  else
-    let elimId := optElimId[1]
-    let elimName ← withRef elimId do resolveGlobalConstNoOverloadWithInfo elimId
-    withRef elimId <| getElimInfo elimName
-
-private def shouldGeneralizeTarget (e : Expr) : MetaM Bool := do
-  if let .fvar fvarId .. := e then
-    return (←  fvarId.getDecl).hasValue -- must generalize let-decls
-  else
-    return true
-
-private def generalizeTargets (exprs : Array Expr) : TacticM (Array Expr) := do
-  if (← withMainContext <| exprs.anyM (shouldGeneralizeTarget ·)) then
-    liftMetaTacticAux fun mvarId => do
-      let (fvarIds, mvarId) ← mvarId.generalize (exprs.map fun expr => { expr })
-      return (fvarIds.map mkFVar, [mvarId])
-  else
-    return exprs
-
-def elabCasesTargets (targets : Array Syntax) : TacticM (Array Expr) :=
-  withMainContext do
-    let args ← targets.mapM fun target => do
-      let hName? := if target[0].isNone then none else some target[0][0].getId
-      let expr ← elabTerm target[1] none
-      return { expr, hName? : GeneralizeArg }
-    if (← withMainContext <| args.anyM fun arg => shouldGeneralizeTarget arg.expr <||> pure arg.hName?.isSome) then
-      liftMetaTacticAux fun mvarId => do
-        let argsToGeneralize ← args.filterM fun arg => shouldGeneralizeTarget arg.expr <||> pure arg.hName?.isSome
-        let (fvarIdsNew, mvarId) ← mvarId.generalize argsToGeneralize
-        let mut result := #[]
-        let mut j := 0
-        for arg in args do
-          if (← shouldGeneralizeTarget arg.expr) || arg.hName?.isSome then
-            result := result.push (mkFVar fvarIdsNew[j]!)
-            j := j+1
-          else
-            result := result.push arg.expr
-        return (result, [mvarId])
-    else
-      return args.map (·.expr)
-
--- # End of duplicate code
-
-def appendMVars (old : Array MVarId) (new : Array MVarId) : TacticM (Array MVarId) := 
-  return old ++ new
-
--- Resembles `evalAlts` in Core Lean
-def getMVarsFromAlts (elimInfo : ElimInfo) (alts : Array (Name × MVarId)) (optPreTac : Syntax) (altsSyntax : Array Syntax)
-    (initialInfo : Info)
-    (numEqs : Nat := 0) (numGeneralized : Nat := 0) (toClear : Array FVarId := #[]) : TacticM (Array MVarId) := do
-  checkAltNames alts altsSyntax
-  let hasAlts := altsSyntax.size > 0
-  if hasAlts then
-    -- default to initial state outside of alts
-    withInfoContext go (pure initialInfo)
-  else go
-where
-  go := do
-    let alts := reorderAlts alts altsSyntax
-    let hasAlts := altsSyntax.size > 0
-    let mut usedWildcard := false
-    let mut subgoals := #[] -- when alternatives are not provided, we accumulate subgoals here
-    let mut altsSyntax := altsSyntax
-
-    -- TODO foreach, add mvar to list, or alts.mapM
-    let mut mvars : List MVarId := []
-    
-    for (altName, altMVarId) in alts do
-      let numFields ← getAltNumFields elimInfo altName
-      let mut isWildcard := false
-      let altStx? ←
-        match altsSyntax.findIdx? (fun alt => getAltName alt == altName) with
-        | some idx =>
-          let altStx := altsSyntax[idx]!
-          altsSyntax := altsSyntax.eraseIdx idx
-          pure (some altStx)
-        | none => match altsSyntax.findIdx? (fun alt => getAltName alt == `_) with
-          | some idx =>
-            isWildcard := true
-            pure (some altsSyntax[idx]!)
-          | none =>
-            pure none
-      match altStx? with
-      | none =>
-        -- Change: Ignore this match, 
-        -- this is probably a match without any alternative syntax, all intro's are inaccessible anyways
-        let mut (_, altMVarId) ← altMVarId.introN numFields
-        match (← Cases.unifyEqs? numEqs altMVarId {}) with
-        | none   => pure () -- alternative is not reachable
-        | some (altMVarId', _) =>
-          (_, altMVarId) ← altMVarId'.introNP numGeneralized
-          for fvarId in toClear do
-            altMVarId ← altMVarId.tryClear fvarId
-          let altMVarIds ← applyPreTac altMVarId
-          if !hasAlts then
-            -- User did not provide alternatives using `|`
-            subgoals := subgoals ++ altMVarIds.toArray
-          else if altMVarIds.isEmpty then
-            pure ()
-          else
-            logError m!"alternative '{altName}' has not been provided"
-            altMVarIds.forM fun mvarId => admitGoal mvarId
-      | some altStx =>
-        (subgoals, usedWildcard, mvars) ← withRef altStx do
-          let unusedAlt :=
-            if isWildcard then
-              pure (#[], usedWildcard, [])
-            else
-              throwError "alternative '{altName}' is not needed"
-          let altVarNames := getAltVarNames altStx
-          let numFieldsToName ← if altHasExplicitModifier altStx then pure numFields else getNumExplicitFields altMVarId numFields
-          if altVarNames.size > numFieldsToName then
-            logError m!"too many variable names provided at alternative '{altName}', #{altVarNames.size} provided, but #{numFieldsToName} expected"
-          let mut (fvarIds, altMVarId) ← altMVarId.introN numFields altVarNames.toList (useNamesForExplicitOnly := !altHasExplicitModifier altStx)
-
-          saveAltVarsInfo altMVarId altStx fvarIds
-          match (← Cases.unifyEqs? numEqs altMVarId {}) with
-          | none => unusedAlt
-          | some (altMVarId', _) =>
-            (_, altMVarId) ← altMVarId'.introNP numGeneralized
-            for fvarId in toClear do
-              altMVarId ← altMVarId.tryClear fvarId
-            let altMVarIds ← applyPreTac altMVarId
-            if altMVarIds.isEmpty then
-              unusedAlt
-            else
-              let mut subgoals := subgoals
-
-              for altMVarId' in altMVarIds do
-                subgoals ← evalAlt altMVarId' altStx subgoals
-              pure (subgoals, usedWildcard || isWildcard, altMVarIds)          
-    if usedWildcard then
-      altsSyntax := altsSyntax.filter fun alt => getAltName alt != `_
-    unless altsSyntax.isEmpty do
-      logErrorAt altsSyntax[0]! "unused alternative"
-    setGoals subgoals.toList
-    -- Change, actually return mvars
-    return mvars.toArray
-  applyPreTac (mvarId : MVarId) : TacticM (List MVarId) :=
-    if optPreTac.isNone then do
-      return [mvarId]
-    else
-      evalTacticAt optPreTac[0] mvarId
-
--- Resembles `evalCases` in Core Lean
-def getMVarsFromCaseMatch (stx : Syntax) : TacticM (Array MVarId) :=
-  match expandCases? stx with
-  | some stxNew => do
-    -- Changed to ignore macro expansion, since evalTactic does not automatically reduce to a correctly nested call to this function
-    trace[Elab.induction] m!"Current implementation ignores macro expansion"
-    return #[]
-  | _ => focus do
-    let targets ← elabCasesTargets stx[1].getSepArgs
-    let optInductionAlts := stx[3]
-    let optPreTac := getOptPreTacOfOptInductionAlts optInductionAlts
-    let alts :=  getAltsOfOptInductionAlts optInductionAlts
-    let targetRef := stx[1]
-    let elimInfo ← withMainContext <| getElimNameInfo stx[2] targets (induction := false)
-    let mvarId ← getMainGoal
-    let initInfo ← mkTacticInfo (← getMCtx) (← getUnsolvedGoals) (← getRef)
-    let tag ← mvarId.getTag
-    mvarId.withContext do
-      let targets ← addImplicitTargets elimInfo targets
-      let result ← withRef targetRef <| mkElimApp elimInfo targets tag
-      let elimArgs := result.elimApp.getAppArgs
-      let targets ← elimInfo.targetsPos.mapM fun i => instantiateMVars elimArgs[i]!
-      let motiveType ← inferType elimArgs[elimInfo.motivePos]!
-      let mvarId ← generalizeTargetsEq mvarId motiveType targets
-      let (targetsNew, mvarId) ← mvarId.introN targets.size
-
-      mvarId.withContext do
-        setMotiveArg mvarId elimArgs[elimInfo.motivePos]!.mvarId! targetsNew
-        mvarId.assign result.elimApp
-
-        -- Changed call to `evalAlts` to modified version that returns `Array MVarId`
-        return (←  getMVarsFromAlts elimInfo result.alts optPreTac alts initInfo (numEqs := targets.size) (toClear := targetsNew))
-
--- Resembles `evalInduction` in Core Lean
--- def 
-def getMVarsFromInductionMatch (stx : Syntax) : TacticM (Array MVarId) := 
-  match expandInduction? stx with
-  | some stxNew => do
-    -- Changed to ignore macro expansion, since evalTactic does not automatically reduce to a correctly nested call to this function
-      trace[Elab.induction] m!"Current implementation ignores macro expansion"
-      return #[]
-  | _ => focus do
-    let optInductionAlts := stx[4]
-    let alts := getAltsOfOptInductionAlts optInductionAlts
-    let targets ← withMainContext <| stx[1].getSepArgs.mapM (elabTerm · none)
-    let targets ← generalizeTargets targets
-    let elimInfo ← withMainContext <| getElimNameInfo stx[2] targets (induction := true)
-    let mvarId ← getMainGoal
-    -- save initial info before main goal is reassigned
-    let initInfo ← mkTacticInfo (← getMCtx) (← getUnsolvedGoals) (← getRef)
-    let tag ← mvarId.getTag
-    mvarId.withContext do
-      let targets ← addImplicitTargets elimInfo targets
-      checkTargets targets
-      let targetFVarIds := targets.map (·.fvarId!)
-      let (n, mvarId) ← generalizeVars mvarId stx targets
-      mvarId.withContext do
-        let result ← withRef stx[1] do -- use target position as reference
-          mkElimApp elimInfo targets tag
-        trace[Elab.induction] "elimApp: {result.elimApp}"
-        let elimArgs := result.elimApp.getAppArgs
-        setMotiveArg mvarId elimArgs[elimInfo.motivePos]!.mvarId! targetFVarIds
-        let optPreTac := getOptPreTacOfOptInductionAlts optInductionAlts
-        mvarId.assign result.elimApp
-
-        -- Changed call to `evalAlts` to modified version that returns `Array MVarId`
-        return (←  getMVarsFromAlts elimInfo result.alts optPreTac alts initInfo (numGeneralized := n) (toClear := targetFVarIds))
-where
-  checkTargets (targets : Array Expr) : MetaM Unit := do
-    let mut foundFVars : FVarIdSet := {}
-    for target in targets do
-      unless target.isFVar do
-        throwError "index in target's type is not a variable (consider using the `cases` tactic instead){indentExpr target}"
-      if foundFVars.contains target.fvarId! then
-        throwError "target (or one of its indices) occurs more than once{indentExpr target}"
-
-def getMVarsFromMatch (oldGoal : MVarId) (matchTactic : TSyntax `tactic) (isInduction : Bool) : TacticM (Array MVarId) := do
-  withoutModifyingState do 
-    match isInduction with
-    | true => return (← getMVarsFromInductionMatch matchTactic.raw)
-    | false => return (← getMVarsFromCaseMatch matchTactic.raw)
-
-end InductionHelper
